theories/TTT.v
@@ -1,91 +1,96 @@
-(** Kearns-Vazirani automata learning
-    https://doi.org/10.7551/mitpress%2F3897.001.0001 *)
+(** TTT automata learning
+    https://doi.org/10.1007/978-3-319-11164-3 *)
 
-From lstar Require Import DFA ListLemmas Teacher RS.
-From Stdlib Require Import List.
-From Stdlib Require Import Lia.
-From Stdlib Require Import PeanoNat.
-From Stdlib Require Import Setoids.Setoid.
+From Stdlib Require Import Lia PeanoNat Bool.
 From Stdlib Require Import Eqdep_dec.
+From lstar Require Import DFA Teacher ListLemmas RS.
 Import ListNotations.
 
-Module KV (s : Symbol) (L : RegularLanguage s) (Tch : Teacher s L).
+Module TTT (s : Symbol) (L : RegularLanguage s) (Tch : Teacher s L).
 Import s L Tch D.
 
-(** A discrimination tree is a binary tree whose internal nodes hold a
-    discriminator suffix and whose leaves hold an access string *)
-Inductive dtree : Type :=
-| Leaf (access : str)
-| Node (discrim : str) (lt rt : dtree).
+(** Trees are now tagged with whether their discriminators are
+    _final_ or _temporary_ *)
+Inductive disc : Type :=
+| Final (e : str)
+| Temp  (e : str).
 
-(** Sifting classifies a string u by descending the tree until it reaches
-    the appropriate access node *)
-Fixpoint sift (t : dtree) (u : str) : str :=
+Definition disc_str (d : disc) : str :=
+    match d with Final e => e | Temp e => e end.
+
+Inductive ttree : Type :=
+| Leaf (access : str)
+| Node (d : disc) (lt rt : ttree).
+
+(** Sifting, as in KV *)
+Fixpoint sift (t : ttree) (u : str) : str :=
     match t with
     | Leaf q => q
-    | Node e lt rt =>
-        if member (u ++ e) then sift lt u else sift rt u
+    | Node d lt rt =>
+        if member (u ++ disc_str d) then sift lt u else sift rt u
     end.
 
-Fixpoint leaves (t : dtree) : list str :=
+Fixpoint leaves (t : ttree) : list str :=
     match t with
     | Leaf q => [q]
     | Node _ lt rt => leaves lt ++ leaves rt
     end.
 
-Fixpoint discriminators (t : dtree) : list str :=
+Fixpoint discriminators (t : ttree) : list disc :=
     match t with
     | Leaf _ => []
-    | Node e lt rt => e :: discriminators lt ++ discriminators rt
+    | Node d lt rt => d :: discriminators lt ++ discriminators rt
     end.
 
-(** Sifting always lands on a leaf of the tree *)
 Lemma sift_in_leaves : forall t u, In (sift t u) (leaves t).
 Proof.
-    induction t0 as [q | e lt IHlt rt IHrt]; intro u; simpl.
+    induction t0; intro u; simpl.
         now left.
-    destruct (member (u ++ e)); auto using in_or_app.
+    destruct (member (u ++ disc_str d)); auto using in_or_app.
 Qed.
 
-(** Tree invariants *)
-
-(** A tree is _consistent_ when every access string sifts to its own leaf *)
-Definition consistent (t : dtree) : Prop :=
+(** Tree invariants, as in KV *)
+Definition consistent (t : ttree) : Prop :=
     forall q, In q (leaves t) -> sift t q = q.
 
-(** A tree is _separated_ when any two distinct leaves are told apart by some
-    discriminator of the tree *)
-Definition separated (t : dtree) : Prop :=
+Definition separated (t : ttree) : Prop :=
     forall u v,
         In u (leaves t) -> In v (leaves t) -> u <> v ->
-        exists e, In e (discriminators t) /\ member (u ++ e) <> member (v ++ e).
+        exists d, In d (discriminators t)
+                /\ member (u ++ disc_str d) <> member (v ++ disc_str d).
 
-(** A tree is _well-formed_ when each node's discriminator bisects the behavior
-    of its two subtrees. Or, every leaf below the [true] branch agrees with the
-    discriminator, every leaf below the [false] branch disagrees *)
-Fixpoint wf' (t : dtree) : Prop :=
+Fixpoint wf' (t : ttree) : Prop :=
     match t with
     | Leaf _ => True
-    | Node e lt rt =>
-        (forall q, In q (leaves lt) -> member (q ++ e) = true) /\
-        (forall q, In q (leaves rt) -> member (q ++ e) = false) /\
+    | Node d lt rt =>
+        (forall q, In q (leaves lt) -> member (q ++ disc_str d) = true) /\
+        (forall q, In q (leaves rt) -> member (q ++ disc_str d) = false) /\
         wf' lt /\ wf' rt
     end.
 Definition wf t := wf' t /\ In nil (leaves t).
+
+(** A discrimination tree is _finalized_ if all of its
+    internal nodes are final *)
+Fixpoint finalized (t : ttree) : Prop :=
+    match t with
+    | Leaf _ => True
+    | Node (Final _) lt rt => finalized lt /\ finalized rt
+    | _ => False
+    end.
 
 Definition mem := mem str_eq.
 
 Lemma sift_mem : forall t u, mem (sift t u) (leaves t) = true.
 Proof. intros. apply mem_In, sift_in_leaves. Qed.
 
-Definition make_dfa (t : dtree) : D.t { q | mem q (leaves t) = true }.
+(** Hypothesis construction, as in KV *)
+Definition make_dfa (t : ttree) : D.t { q | mem q (leaves t) = true }.
     set (state := { q | mem q (leaves t) = true }).
     assert (initial : state). {
         exists (sift t nil). apply sift_mem. }
     assert (transition : state -> s.t -> state). {
         intros q a. exists (sift t (proj1_sig q ++ [a])). apply sift_mem. }
     set (accept := fun (q : state) => member (proj1_sig q)).
-    (* enumerate the leaves as the carrier list, via mem-proofs *)
     assert (mempf : forall x, In x (leaves t) -> mem x (leaves t) = true)
         by (intros x Hx; now apply mem_In).
     set (ls := list_with_proof (leaves t) (fun q => mem q (leaves t) = true) mempf).
@@ -147,39 +152,37 @@ Qed.
 
 (** Set up Rivest-Schapire counterexample analysis *)
 Module RSS <: RS_Setup s L Tch.
-  Definition obt := { o : dtree | wf o }.
+  Definition obt := { o : ttree | wf o }.
   Definition P (o : obt) (q : str) : Prop := mem q (leaves (proj1_sig o)) = true.
   Definition make_dfa (o : obt) : D.t { q | P o q } := make_dfa (proj1_sig o).
 
   Lemma eps_in_H : forall (o : obt),
       proj1_sig (make_dfa o).(initial _) = [].
   Proof.
-    intros (t & Hwf). unfold make_dfa, KV.make_dfa. simpl.
+    intros (t & Hwf). unfold make_dfa, TTT.make_dfa. simpl.
     apply (wf_consistent t Hwf). now destruct Hwf.
   Qed.
 
   Lemma acc_correct : forall (o : obt) q,
       accept _ (make_dfa o) q = member (proj1_sig q).
   Proof.
-    intros (t & Hwf) q. unfold make_dfa, KV.make_dfa. reflexivity.
+    intros (t & Hwf) q. unfold make_dfa, TTT.make_dfa. reflexivity.
   Qed.
 End RSS.
 
 Module RSan := RS s L Tch RSS.
 Import RSan.
 
-(** Replace the leaf whose access string is [target] by an internal node discriminating
-    on e *)
-Fixpoint split_leaf (t : dtree) (target e q_new : str) : dtree :=
+Fixpoint split_leaf (t : ttree) (target e q_new : str) : ttree :=
     match t with
     | Leaf q =>
         if str_eq q target
         then if member (q ++ e)
-             then Node e (Leaf q)     (Leaf q_new)
-             else Node e (Leaf q_new) (Leaf q)
+             then Node (Temp e) (Leaf q)     (Leaf q_new)
+             else Node (Temp e) (Leaf q_new) (Leaf q)
         else Leaf q
-    | Node e' lt rt =>
-        Node e' (split_leaf lt target e q_new) (split_leaf rt target e q_new)
+    | Node d lt rt =>
+        Node d (split_leaf lt target e q_new) (split_leaf rt target e q_new)
     end.
 
 Lemma split_leaves_fwd : forall t target e q_new x,
@@ -241,19 +244,6 @@ Proof.
     now apply split_leaves_pres.
 Qed.
 
-Lemma split_discriminators_incl : forall t target e q_new,
-    incl (discriminators t) (discriminators (split_leaf t target e q_new)).
-Proof.
-    induction t0 as [q | e' lt IHlt rt IHrt]; intros; simpl.
-    - destruct (str_eq q target); [destruct (member (q ++ e)); simpl |];
-        intros x Hx; inversion Hx.
-    - intros x Hx. simpl in Hx. destruct Hx as [-> | Hx].
-          now left.
-      right. apply in_or_app. apply in_app_or in Hx. destruct Hx.
-        left. now apply IHlt.
-        right. now apply IHrt.
-Qed.
-
 (** A well-oriented split preserves distinctness of leaves: [target] occurs once
     and [q_new] is fresh, so replacing the former by the pair adds no
     duplicates *)
@@ -292,38 +282,38 @@ Proof.
         now apply (NoDup_app_disj _ _ HND x Hx).
 Qed.
 
+
 Lemma consistent_NoDup_wf' : forall t,
     NoDup (leaves t) -> consistent t -> wf' t.
 Proof.
-    induction t0 as [q | e lt IHlt rt IHrt]; intros HND Hcons; [exact I |].
+    induction t0 as [q | d lt IHlt rt IHrt]; intros HND Hcons; [exact I |].
     simpl in HND.
     pose proof (NoDup_app_l _ _ HND) as NDl.
     pose proof (NoDup_app_r _ _ HND) as NDr.
     assert (Hdisj : forall x, In x (leaves lt) -> ~ In x (leaves rt))
         by now apply NoDup_app_disj.
-    (* the left subtree's leaves agree with the discriminator *)
-    assert (Hl : forall q, In q (leaves lt) -> member (q ++ e) = true). {
-        intros q Hq. destruct (member (q ++ e)) eqn:E; [reflexivity |]. exfalso.
-        assert (Hsc : sift (Node e lt rt) q = q)
+    assert (Hl : forall q, In q (leaves lt) -> member (q ++ disc_str d) = true). {
+        intros q Hq. destruct (member (q ++ disc_str d)) eqn:E; [reflexivity |].
+        exfalso.
+        assert (Hsc : sift (Node d lt rt) q = q)
             by (apply Hcons; simpl; apply in_or_app; now left).
         simpl in Hsc. rewrite E in Hsc.
         apply (Hdisj q Hq). rewrite <- Hsc. apply sift_in_leaves. }
-    (* the right subtree's leaves disagree with it *)
-    assert (Hr : forall q, In q (leaves rt) -> member (q ++ e) = false). {
-        intros q Hq. destruct (member (q ++ e)) eqn:E; [| reflexivity]. exfalso.
-        assert (Hsc : sift (Node e lt rt) q = q)
+    assert (Hr : forall q, In q (leaves rt) -> member (q ++ disc_str d) = false). {
+        intros q Hq. destruct (member (q ++ disc_str d)) eqn:E; [| reflexivity].
+        exfalso.
+        assert (Hsc : sift (Node d lt rt) q = q)
             by (apply Hcons; simpl; apply in_or_app; now right).
         simpl in Hsc. rewrite E in Hsc.
         apply (Hdisj q); [rewrite <- Hsc; apply sift_in_leaves | assumption]. }
-    (* and the subtrees are themselves consistent *)
     assert (Cl : consistent lt). {
         intros q Hq.
-        assert (Hsc : sift (Node e lt rt) q = q)
+        assert (Hsc : sift (Node d lt rt) q = q)
             by (apply Hcons; simpl; apply in_or_app; now left).
         simpl in Hsc. now rewrite (Hl q Hq) in Hsc. }
     assert (Cr : consistent rt). {
         intros q Hq.
-        assert (Hsc : sift (Node e lt rt) q = q)
+        assert (Hsc : sift (Node d lt rt) q = q)
             by (apply Hcons; simpl; apply in_or_app; now right).
         simpl in Hsc. now rewrite (Hr q Hq) in Hsc. }
     simpl. repeat split; auto.
@@ -345,7 +335,7 @@ Proof.
       (* the new node's two singleton leaves witness orientation *)
       destruct (member (q ++ e)) eqn:Em; repeat split; auto;
       intros x Hx; destruct Hx as [Hx|[]]; subst x; subst; easy ||
-      now destruct (member (q_new ++ e)).
+      (simpl; now destruct (member (q_new ++ e))).
     - simpl in Hwf. destruct Hwf as (Hl & Hr & Wl & Wr).
       simpl in HinT, Hfresh. apply in_app_or in HinT. simpl.
       assert (Hfl : ~ In q_new (leaves lt))
@@ -358,8 +348,8 @@ Proof.
             by (intro H; pose proof (Hl target Hin); pose proof (Hr target H);
                 congruence).
         (* q_new sifts toward the left subtree as well *)
-        assert (Hqe' : member (q_new ++ e') = true). {
-            destruct (member (q_new ++ e')) eqn:E; [reflexivity |].
+        assert (Hqe' : member (q_new ++ disc_str e') = true). {
+            destruct (member (q_new ++ disc_str e')) eqn:E; [reflexivity |].
             destruct Hnr.
             assert (sift rt q_new = target) by (simpl in Hsift; now rewrite E in Hsift).
             rewrite <- H. apply sift_in_leaves. }
@@ -372,8 +362,8 @@ Proof.
         assert (Hnl : ~ In target (leaves lt))
             by (intro H; pose proof (Hl target H); pose proof (Hr target Hin);
                 congruence).
-        assert (Hqe' : member (q_new ++ e') = false). {
-            destruct (member (q_new ++ e')) eqn:E; [| reflexivity].
+        assert (Hqe' : member (q_new ++ disc_str e') = false). {
+            destruct (member (q_new ++ disc_str e')) eqn:E; [| reflexivity].
             destruct Hnl.
             assert (sift lt q_new = target) by (simpl in Hsift; now rewrite E in Hsift).
             rewrite <- H. apply sift_in_leaves. }
@@ -384,11 +374,9 @@ Proof.
         intros x Hx. apply split_leaves_fwd in Hx. destruct Hx as [-> | Hx]; auto.
 Qed.
 
-(** Given a tree whose hypothesis mispredicts on a counterexample w, we can find
-    a leaf [target] and a fresh discriminator e such that splitting [target] on
-    e yields a still well-formed tree *)
+
 Theorem find_split :
-    forall (t : dtree) (w : str)
+    forall (t : ttree) (w : str)
            (Heps : In nil (leaves t))
            (Hcons : consistent t)
            (HND : NoDup (leaves t))
@@ -406,15 +394,12 @@ Proof.
     assert (Hwf : wf t) by (split; [ now apply consistent_NoDup_wf' | easy ]).
     destruct (partition_binary (exist _ t Hwf) w Hce)
       as (k & Kcorrect & SKincorrect).
-    (* The breakpoint lies strictly inside w, since beyond [length w] both
-       prefixes coincide with all of w *)
-    assert (Hlt : k < length w). {
-        destruct (Nat.le_gt_cases (length w) k) as [Hle |]; [| assumption].
+    assert (Hlt : k < List.length w). {
+        destruct (Nat.le_gt_cases (List.length w) k) as [Hle |]; [| assumption].
         destruct SKincorrect. unfold correct, pi in *.
         rewrite firstn_all2, skipn_all2, app_nil_r by lia.
         now rewrite firstn_all2, skipn_all2, app_nil_r in Kcorrect by lia.
     }
-    (* Retrieve w[k] *)
     assert {wk | nth_error w k = Some wk}. {
         destruct (nth_error w k) eqn:E.
             now exists t0.
@@ -429,13 +414,10 @@ Proof.
     set (o := exist wf t Hwf : RSS.obt).
     set (qk1 := pi o w k ++ [wk]).
     exists (sift t qk1), (skipn (S k) w), qk1.
-    (* One step of the hypothesis advances from p_k to the leaf [qk1] sifts to *)
     assert (HSk : pi o w (S k) = sift t qk1). {
         unfold pi, qk1, run, make_dfa. rewrite Hfirstn, fold_left_app.
         reflexivity.
     }
-    (* From correctness at k and incorrectness at (S k), the extension and the
-       leaf it sifts to are told apart by the suffix e *)
     assert (Hgk : member (qk1 ++ skipn (S k) w) = member w). {
         unfold correct in Kcorrect.
         rewrite (skipn_S_wk _ _ _ _ Hwk) in Kcorrect.
@@ -456,16 +438,14 @@ Proof.
     repeat split; auto using split_leaves_pres.
 Defined.
 
-(** Each counterexample adds exactly one state *)
 Lemma split_leaf_count : forall t target e q_new,
     NoDup (leaves t) -> In target (leaves t) -> ~ In q_new (leaves t) ->
-    length (leaves (split_leaf t target e q_new)) = S (length (leaves t)).
+    List.length (leaves (split_leaf t target e q_new)) = S (List.length (leaves t)).
 Proof.
     intros t target e q_new HND HinT Hfresh.
     assert (ND' : NoDup (leaves (split_leaf t target e q_new)))
         by now apply split_NoDup.
     assert (NDc : NoDup (q_new :: leaves t)) by now constructor.
-    (* the split tree and [q_new :: leaves t] have the same elements *)
     assert (I1 : incl (leaves (split_leaf t target e q_new)) (q_new :: leaves t)). {
         intros x Hx. apply split_leaves_fwd in Hx. destruct Hx as [-> | Hx]; now constructor.
     }
@@ -473,9 +453,9 @@ Proof.
         intros x [-> | Hx];
             [now apply split_q_new_in | now apply split_leaves_pres].
     }
-    pose proof (NoDup_incl_length ND' I1) as L1.
-    pose proof (NoDup_incl_length NDc I2) as L2.
-    simpl in L1, L2. lia.
+    pose proof (NoDup_incl_length ND' I1) as Ln1.
+    pose proof (NoDup_incl_length NDc I2) as Ln2.
+    simpl in Ln1, Ln2. lia.
 Qed.
 
 Lemma make_dfa_minimal : forall t,
@@ -497,22 +477,23 @@ Proof.
   assert (Hinj : forall u v, In u (leaves t) -> In v (leaves t) ->
                  u <> v -> f u <> f v). {
     intros u v Hu Hv Huv Hf.
-    destruct (Hsep u v Hu Hv Huv) as (e & He & Hdiff).
+    destruct (Hsep u v Hu Hv Huv) as (d & Hd & Hdiff).
     apply Hdiff.
     assert (Hsplit : forall x,
-              D.accept_string dfa' (x ++ e)
-              = dfa'.(D.accept _) (fold_left dfa'.(D.transition _) e (f x)))
+              D.accept_string dfa' (x ++ disc_str d)
+              = dfa'.(D.accept _) (fold_left dfa'.(D.transition _) (disc_str d) (f x)))
       by (intro x; unfold D.accept_string, D.run, f; now rewrite fold_left_app).
-    assert (Hacc : D.accept_string dfa' (u ++ e) = D.accept_string dfa' (v ++ e))
+    assert (Hacc : D.accept_string dfa' (u ++ disc_str d)
+                 = D.accept_string dfa' (v ++ disc_str d))
       by (rewrite !Hsplit; unfold f in *; now rewrite Hf).
-    destruct (member (u ++ e)) eqn:Mu, (member (v ++ e)) eqn:Mv;
+    destruct (member (u ++ disc_str d)) eqn:Mu, (member (v ++ disc_str d)) eqn:Mv;
       try reflexivity; exfalso.
-    - assert (D.accept_string dfa' (u ++ e) = true) by (now apply H_encodes).
-      assert (D.accept_string dfa' (v ++ e) = true) by (now rewrite <- Hacc).
-      assert (member (v ++ e) = true) by (now apply H_encodes). congruence.
-    - assert (D.accept_string dfa' (v ++ e) = true) by (now apply H_encodes).
-      assert (D.accept_string dfa' (u ++ e) = true) by (now rewrite Hacc).
-      assert (member (u ++ e) = true) by (now apply H_encodes). congruence. }
+    - assert (D.accept_string dfa' (u ++ disc_str d) = true) by (now apply H_encodes).
+      assert (D.accept_string dfa' (v ++ disc_str d) = true) by (now rewrite <- Hacc).
+      assert (member (v ++ disc_str d) = true) by (now apply H_encodes). congruence.
+    - assert (D.accept_string dfa' (v ++ disc_str d) = true) by (now apply H_encodes).
+      assert (D.accept_string dfa' (u ++ disc_str d) = true) by (now rewrite Hacc).
+      assert (member (u ++ disc_str d) = true) by (now apply H_encodes). congruence. }
   rewrite <- (length_map f (leaves t)).
   apply NoDup_incl_length.
   - clear - HND Hinj.
@@ -523,51 +504,44 @@ Proof.
       destruct (str_eq x y) as [e0|n0]; [now symmetry|].
       exfalso. apply (Hinj x y); [now left | now right | assumption | now symmetry].
     + apply IH; auto. intros u v Hu Hv. apply Hinj; now right.
-  - (* every mapped state is a real state of dfa' *)
-    intros st Hst. apply in_map_iff in Hst.
+  - intros st Hst. apply in_map_iff in Hst.
     destruct Hst as (q & <- & _). unfold f. apply D.run_in_states.
 Qed.
 
 Lemma le_min : forall t,
     wf t ->
-    length (leaves t) <= num_states_in_minimal.
+    List.length (leaves t) <= num_states_in_minimal.
 Proof.
   intro t. intro Hwf.
-  destruct L.exists_dfa as (state_m & D & [Denc Minimal] & Len).
-  (* It suffices to bound leaves by D's state count *)
-  enough (Hle : List.length (leaves t) <= List.length (D.states state_m D)) by lia.
+  destruct L.exists_dfa as (state_m & Dm & [Denc Minimal] & Len).
+  enough (Hle : List.length (leaves t) <= List.length (D.states state_m Dm)) by lia.
   pose proof (wf_separated _ Hwf) as Hsep.
   pose proof (wf_NoDup _ Hwf) as HND.
-  set (f := fun q => D.run D q).
-  (* f is injective on the leaves *)
+  set (f := fun q => D.run Dm q).
   assert (Hinj : forall u v, In u (leaves t) -> In v (leaves t) ->
                  u <> v -> f u <> f v). {
     intros u v Hu Hv Huv Hf.
-    (* Some discriminator e of t tells u and v apart *)
-    destruct (Hsep u v Hu Hv Huv) as (e & He & Hdiff).
-    (* But equal runs make u and v agree on every suffix, including e *)
+    destruct (Hsep u v Hu Hv Huv) as (d & Hd & Hdiff).
     apply Hdiff.
     assert (Hsplit : forall x,
-              D.accept_string D (x ++ e)
-              = D.(D.accept _) (fold_left D.(D.transition _) e (f x))). {
+              D.accept_string Dm (x ++ disc_str d)
+              = Dm.(D.accept _) (fold_left Dm.(D.transition _) (disc_str d) (f x))). {
       intro x. unfold D.accept_string, D.run, f. now rewrite fold_left_app. }
-    assert (Hacc : D.accept_string D (u ++ e) = D.accept_string D (v ++ e)). {
+    assert (Hacc : D.accept_string Dm (u ++ disc_str d)
+                 = D.accept_string Dm (v ++ disc_str d)). {
       rewrite Hsplit. unfold f in *. now rewrite Hf. }
-    (* Transport the acceptance equality back to membership via Denc *)
-    destruct (member (u ++ e)) eqn:Mu, (member (v ++ e)) eqn:Mv;
+    destruct (member (u ++ disc_str d)) eqn:Mu, (member (v ++ disc_str d)) eqn:Mv;
       try reflexivity; exfalso.
-    - assert (D.accept_string D (u ++ e) = true) by (now apply Denc).
-      assert (D.accept_string D (v ++ e) = true) by (now rewrite <- Hacc).
-      assert (member (v ++ e) = true) by (now apply Denc). congruence.
-    - assert (D.accept_string D (v ++ e) = true) by (now apply Denc).
-      assert (D.accept_string D (u ++ e) = true) by (now rewrite Hacc).
-      assert (member (u ++ e) = true) by (now apply Denc). congruence.
+    - assert (D.accept_string Dm (u ++ disc_str d) = true) by (now apply Denc).
+      assert (D.accept_string Dm (v ++ disc_str d) = true) by (now rewrite <- Hacc).
+      assert (member (v ++ disc_str d) = true) by (now apply Denc). congruence.
+    - assert (D.accept_string Dm (v ++ disc_str d) = true) by (now apply Denc).
+      assert (D.accept_string Dm (u ++ disc_str d) = true) by (now rewrite Hacc).
+      assert (member (u ++ disc_str d) = true) by (now apply Denc). congruence.
   }
-  (* An injection from leaves into D's states bounds the lengths *)
   rewrite <- (length_map f (leaves t)).
   apply NoDup_incl_length.
-  - (* map f (leaves t) is duplicate-free, by injectivity of f on the leaves *)
-    clear - HND Hinj.
+  - clear - HND Hinj.
     induction (leaves t) as [| x xs IH]; [constructor|].
     apply NoDup_cons_iff in HND. destruct HND as [Hnin NDxs]. constructor.
     + intro HIn. apply in_map_iff in HIn. destruct HIn as (y & Hfy & Hyin).
@@ -575,12 +549,11 @@ Proof.
         exfalso. apply (Hinj x y); [now left | now right | exact n | now symmetry]. }
       subst y; contradiction.
     + apply IH; auto. intros u v Hu Hv. apply Hinj; now right.
-  - (* every mapped state is an actual state of D *)
-    intros st Hst. apply in_map_iff in Hst.
+  - intros st Hst. apply in_map_iff in Hst.
     destruct Hst as (q & <- & _). unfold f. apply D.run_in_states.
 Qed.
 
-Lemma full_states_no_ce : forall (t : dtree),
+Lemma full_states_no_ce : forall (t : ttree),
     wf t ->
     L.num_states_in_minimal <= List.length (leaves t) ->
     equiv_query _ (make_dfa t) = None.
@@ -598,39 +571,276 @@ Proof.
     pose proof (split_leaf_count t target e q_new HND In_target NIn_qnew) as Hcount.
     assert (wf (split_leaf t target e q_new)) by now split.
     pose proof (le_min _ H) as Hcap.
-    (* Hcap : length (leaves (split_leaf t target e q_new)) <= num_states_in_minimal *)
     rewrite Hcount in Hcap.
-    (* Hcap : S (length (leaves t)) <= num_states_in_minimal *)
     lia.
 Qed.
 
-(** The main KV implementation. Adds one state per counterexample *)
-Fixpoint kv_learn (fuel : nat) (t : dtree)
-                  (LE : L.num_states_in_minimal - List.length (leaves t) <= fuel)
-                  (Hwf : wf t)
+Section Finalize.
+  Definition bisects e l r : bool :=
+    (forallb (fun q => member (q ++ e)) (leaves l)) &&
+    (forallb (fun q => negb (member (q ++ e))) (leaves r)).
+
+  (* All suffixes of a string [e] *)
+  Fixpoint suffixes (e : str) : list str :=
+    e :: match e with
+         | [] => []
+         | _ :: e' => suffixes e'
+         end.
+
+  (** Among the suffixes of [e], pick the SHORTEST that bisects [l]/[r].
+      If none does, fall back to [e]. *)
+  Definition choose (e : str) (l r : ttree) : str :=
+    match find (fun e' => bisects e' l r) (rev (suffixes e)) with
+    | Some e' => e'
+    | None    => e
+    end.
+
+  Fixpoint finalize (t : ttree) : ttree :=
+    match t with
+    | Leaf q => Leaf q
+    | Node (Final e) lt rt => Node (Final e) (finalize lt) (finalize rt)
+    | Node (Temp e) lt rt =>
+        let lt' := finalize lt in
+        let rt' := finalize rt in
+        Node (Final (choose e lt' rt')) lt' rt'
+    end.
+
+  (** Finalization preserves the leaf set *)
+  Lemma finalize_leaves : forall t, leaves (finalize t) = leaves t.
+  Proof.
+    induction t0 as [q | d lt IHlt rt IHrt]; simpl.
+        reflexivity.
+    destruct d; simpl; now rewrite IHlt, IHrt.
+  Qed.
+
+  (** [finalize] finalizes *)
+  Lemma finalize_finalized : forall t, finalized (finalize t).
+  Proof.
+    induction t0 as [q | d lt IHlt rt IHrt]; simpl.
+        exact I.
+    destruct d; simpl; repeat split; auto.
+  Qed.
+
+  Lemma in_bigger_leaves_impl_in_smaller_leaves :
+    forall s d l r,
+    In s (leaves (Node d l r)) -> In s (leaves l) \/ In s (leaves r).
+  Proof.
+    intros. simpl in H. now apply in_app_or in H.
+  Qed.
+
+  Lemma wf_bisects_impl_bisects :
+    forall e lt rt,
+        (forall q : str, In q (leaves lt) -> member (q ++ e) = true) ->
+        (forall q : str, In q (leaves rt) -> member (q ++ e) = false) ->
+        bisects e lt rt = true.
+  Proof.
+    intros.
+    unfold bisects. apply andb_true_iff. split;
+        apply forallb_forall; intros; eauto.
+    specialize (H0 _ H1). now rewrite H0.
+  Qed.
+
+  (** Conversely, a [bisects] flag gives back the two block-classification
+      facts. Used to turn [choose]'s output into routing information. *)
+  Lemma bisects_impl_clauses :
+    forall e lt rt,
+      bisects e lt rt = true ->
+      (forall q, In q (leaves lt) -> member (q ++ e) = true) /\
+      (forall q, In q (leaves rt) -> member (q ++ e) = false).
+  Proof.
+    unfold bisects. intros e lt rt H. apply andb_true_iff in H as [HL HR].
+    rewrite forallb_forall in HL, HR. split.
+    - intros q Hq. now apply HL.
+    - intros q Hq. specialize (HR q Hq). now apply negb_true_iff in HR.
+  Qed.
+
+  (** Every suffix in [suffixes e] is no longer than [e]. *)
+  Lemma suffixes_length : forall e e',
+    In e' (suffixes e) -> List.length e' <= List.length e.
+  Proof.
+    induction e as [| a e IH]; intros e' Hin; simpl in Hin.
+    - destruct Hin as [<- | []]. reflexivity.
+    - destruct Hin as [<- | Hin].
+      + reflexivity.
+      + simpl. apply le_S. now apply IH.
+  Qed.
+
+  (** Bisecting input gives a bisecting, no-longer output *)
+  Lemma choose_correct : forall e l r,
+    bisects e l r = true ->
+    bisects (choose e l r) l r = true /\
+    List.length (choose e l r) <= List.length e.
+  Proof.
+    intros e l r He. unfold choose.
+    destruct (find (fun e' => bisects e' l r) (rev (suffixes e))) eqn:F.
+    - apply find_some in F as [Hin Hbis].
+      apply in_rev in Hin. auto using suffixes_length.
+    - now split.
+  Qed.
+
+  (** CHOOSE actually shortens when a proper suffix bisects: if some suffix
+      strictly shorter than [e] bisects, the chosen discriminator is strictly
+      shorter. (Optional certification of real shortening.) *)
+  Lemma choose_shortens : forall e l r e0,
+    In e0 (suffixes e) ->
+    bisects e0 l r = true ->
+    List.length (choose e l r) <= List.length e0.
+  Proof.
+    intros e l r e0 Hin Hbis. unfold choose.
+    destruct (find (fun e' => bisects e' l r) (rev (suffixes e))) eqn:F.
+    - apply find_some in F as [Hin' _].
+      apply in_rev in Hin'.
+      admit.
+    - exfalso.
+      assert (Hin_rev : In e0 (rev (suffixes e))) by
+        now apply -> in_rev.
+      pose proof (find_none _ _ F e0 Hin_rev) as Hf. simpl in Hf.
+      congruence.
+  Admitted.
+
+  (** Finalization preserves well-formedness *)
+  Lemma finalize_preserves_wf :
+    forall t, wf t -> wf (finalize t).
+  Proof.
+    intros t H. destruct H as [H Heps]. unfold wf. split;
+        [clear Heps | now rewrite finalize_leaves].
+    induction t as [q | d lt IHlt rt IHrt]; simpl in *.
+        exact I.
+    destruct H as (DL & DR & Hwfl & Hwfr).
+    rewrite <- (finalize_leaves lt) in DL.
+    rewrite <- (finalize_leaves rt) in DR.
+    destruct d; simpl. repeat split; auto.
+    assert (Hbis : bisects e (finalize lt) (finalize rt) = true)
+        by now apply wf_bisects_impl_bisects.
+    destruct (choose_correct e (finalize lt) (finalize rt) Hbis) as [Hchb _].
+    apply bisects_impl_clauses in Hchb as [HL HR].
+    repeat split; auto.
+  Qed.
+
+  Lemma choose_routes_agree_leaves : forall e l r u,
+    bisects e l r = true ->
+    In u (leaves l) \/ In u (leaves r) ->
+    member (u ++ choose e l r) = member (u ++ e).
+  Proof.
+    intros e l r u He Hu.
+    destruct (choose_correct e l r He) as [Hchb _].
+    apply bisects_impl_clauses in He as [HLe HRe].
+    apply bisects_impl_clauses in Hchb as [HLc HRc].
+    destruct Hu as [Hu | Hu].
+    - now rewrite (HLe u Hu), (HLc u Hu).
+    - now rewrite (HRe u Hu), (HRc u Hu).
+  Qed.
+
+  Lemma finalize_sift_agree_leaves :
+    forall t u, wf t -> In u (leaves t) -> sift (finalize t) u = sift t u.
+  Proof.
+    intros t u H. destruct H as [H _].
+    induction t as [q | d lt IHlt rt IHrt]; intro Hu; simpl in *.
+        reflexivity.
+    destruct H as (DL & DR & Hwfl & Hwfr).
+    apply in_app_or in Hu.
+    assert (Hbis : bisects (disc_str d) (finalize lt) (finalize rt) = true). {
+        apply wf_bisects_impl_bisects;
+        intros q Hq; rewrite finalize_leaves in Hq; auto. }
+    destruct d; simpl in *.
+    - destruct (member (u ++ e)) eqn:M; destruct Hu as [Hu | Hu]; auto.
+      admit. admit.
+    - assert (Hroute : member (u ++ choose e (finalize lt) (finalize rt))
+                       = member (u ++ e)). {
+        apply choose_routes_agree_leaves with (l := finalize lt) (r := finalize rt).
+            assumption.
+        now repeat rewrite !finalize_leaves. }
+      rewrite Hroute.
+      destruct (member (u ++ e)) eqn:M; destruct Hu as [Hu | Hu]; auto.
+      admit. admit.
+  Admitted.
+
+  (** Every run-reachable state is a leaf, hence sift-agreement applies along a
+      whole run *)
+  Lemma finalize_run_agree : forall t w,
+    wf t ->
+    proj1_sig (run (make_dfa (finalize t)) w) = proj1_sig (run (make_dfa t) w).
+  Proof.
+    intros t w Hwf.
+    induction w as [| a w IH] using rev_ind.
+    - unfold run, make_dfa; simpl.
+      apply finalize_sift_agree_leaves; now destruct Hwf.
+    - unfold run, make_dfa in *; simpl in *.
+      repeat rewrite fold_left_app; simpl.
+      rewrite finalize_sift_agree_leaves; auto.
+      now rewrite IH.
+      admit.
+  Admitted.
+
+  (** The finalized DFA encodes the same language *)
+  Lemma finalize_make_dfa_agree :
+    forall t w, wf t ->
+      accept_string (make_dfa (finalize t)) w = accept_string (make_dfa t) w.
+  Proof.
+    intros t w H. unfold accept_string, accept.
+    change (member (proj1_sig (run (make_dfa (finalize t)) w))
+            = member (proj1_sig (run (make_dfa t) w))).
+    now rewrite finalize_run_agree.
+  Qed.
+
+  (** Every finalized discriminator is no longer than its origin *)
+  Lemma choose_length : forall e l r,
+    List.length (choose e l r) <= List.length e.
+  Proof.
+    intros e l r. unfold choose.
+    destruct (find (fun e' => bisects e' l r) (rev (suffixes e))) eqn:F;
+        [|reflexivity].
+    apply find_some in F as [Hin _]. apply in_rev in Hin.
+    now apply suffixes_length.
+  Qed.
+
+  Lemma finalize_length_bound :
+  forall t,
+    Forall (fun d' => exists d, In d (discriminators t) /\
+                          List.length (disc_str d') <= List.length (disc_str d))
+           (discriminators (finalize t)).
+  Proof.
+    intros t.
+    induction t as [q | d lt IHlt rt IHrt]; simpl in *.
+        constructor.
+    destruct d; simpl.
+    - constructor.
+        eexists. split; auto.
+      apply Forall_app. split.
+      -- eapply Forall_impl; [| eassumption].
+         intros d' (d & Hin & Hle). exists d. split; [| assumption].
+         right. apply in_or_app. now left.
+      -- eapply Forall_impl; [| eassumption].
+         intros d' (d & Hin & Hle). exists d. split; [| assumption].
+         right. apply in_or_app. now right.
+    - constructor.
+        eexists. split; [now left |]. simpl.
+        apply choose_length.
+      apply Forall_app. split.
+      -- eapply Forall_impl; [| eassumption].
+         intros d' (d & Hin & Hle). exists d. split; [| assumption].
+         right. apply in_or_app. now left.
+      -- eapply Forall_impl; [| eassumption].
+         intros d' (d & Hin & Hle). exists d. split; [| assumption].
+         right. apply in_or_app. now right.
+  Qed.
+
+End Finalize.
+
+Section Learner.
+  Definition ttt_step (t : ttree) (target e q_new : str) : ttree.
+  Admitted.
+
+  Definition ttt_learn (fuel : nat) (t : ttree)
+                     (LE : L.num_states_in_minimal - List.length (leaves t) <= fuel)
+                     (Hwf : wf t)
     : { St : Type & {d : D.t St | minimal d} }.
-    destruct (equiv_query _ (make_dfa t)) eqn:Heq.
-    - (* counterexample *)
-        destruct fuel as [| n].
-        -- assert (forall x y, x - y <= 0 -> x - y = 0) by lia. apply H in LE. clear H.
-           apply Nat.sub_0_le, full_states_no_ce in LE; auto.
-           rewrite Heq in LE. discriminate.
-        -- assert (Hce : accept_string (make_dfa t) s <> member s)
-                by now apply equiv_query_ce.
-            pose proof Hwf as Hwf'.
-            destruct Hwf' as (Hwf' & Heps).
-            destruct (find_split t s Heps (wf_consistent t Hwf) (wf_NoDup t Hwf) Hce)
-                as (target & e & q_new & HinT & Hfresh & Hdiff & Hwf'' & Heps').
-            enough (num_states_in_minimal - List.length (leaves (split_leaf t target e q_new)) <= n).
-            eapply (kv_learn n (split_leaf t target e q_new) H (conj Hwf'' Heps')).
-            pose proof (split_leaf_count t target e q_new
-                          (wf_NoDup t Hwf) HinT Hfresh) as Hcount.
-            rewrite Hcount. lia.
-    - eexists. exists (make_dfa t). apply (make_dfa_minimal t Hwf Heq).
-Defined.
+  Proof.
+  Admitted.
 
-(** The learner is seeded with a trivially well-formed tree *)
-Definition kv (_ : unit) : { St : Type & {d : D.t St | minimal d} } :=
-    kv_learn num_states_in_minimal (Leaf nil) ltac:(lia) (conj I (or_introl eq_refl)).
+  Definition ttt (_ : unit) : { St : Type & {d : D.t St | minimal d} } :=
+    ttt_learn num_states_in_minimal (Leaf nil) ltac:(lia) (conj I (or_introl eq_refl)).
 
-End KV.
+End Learner.
+
+End TTT.
