README.md
@@ -6,6 +6,7 @@ A collection of formally-verified implementations of [automata learning](https:/
 | --- | --- | --- |
 | L* | [Angluin, 1987](https://doi.org/10.1016/0890-5401(87)90052-6), [Lecture Notes](https://www.tifr.res.in/~shibashis.guha/courses/diwali2021/L-starMalharManagoli.pdf) | [Lstar.v](theories/Lstar.v) |
 | Kearns-Vazirani | [Kearns-Vazirani, 1994](https://doi.org/10.7551/mitpress/3897.003.0009), [Balle, 2010](https://borjaballe.github.io/papers/zulu10.pdf) | [KV.v](theories/KV.v) |
+| TTT | [Isberner et al., 2014](https://doi.org/10.1007/978-3-319-11164-3) | [TTT.v](theories/TTT.v) |
 
 [These notes](https://www.overleaf.com/read/jbftmjdhmyjd#a32216) summarize each of the main proof arguments and algorithm designs.
 
